theories/iris/helpers/reduce_det/reduce_det_local.v
@@ -2,6 +2,8 @@ From mathcomp Require Import ssreflect eqtype seq ssrbool.
 From stdpp Require Import base list.
 From Wasm.iris.helpers.prelude Require Export iris_reduce_det_prelude iris_split_reduce.
 
+Set Bullet Behavior "Strict Subproofs".
+
 Lemma local_det s f es s' f' es' ws2 n f0 f2 es2 nnn:
   (∀ (f f2 f1 : frame) (es2 es1 es : seq.seq administrative_instruction),
     reduce s f es s' f1 es1
@@ -21,110 +23,172 @@ Proof.
   rewrite <- (app_nil_l [AI_local n f es]) in Heqes0.
   induction Hred2 ; (try by inversion Heqes0) ;
     try by apply app_inj_tail in Heqes0 as [_ Habs] ; inversion Habs.
-  { destruct H ; (try by inversion Heqes0) ;
-      try by apply app_inj_tail in Heqes0 as [_ Habs] ; inversion Habs.
-    - inversion Heqes0 ; subst. exfalso ; values_no_reduce.
-    - inversion Heqes0 ; subst.
-      exfalso ; by apply (test_no_reduce_trap _ _ _ _ _ Hred1).
-    - { inversion Heqes0 ; subst.
-        induction Hred1 ;
-          (try by simple_filled H1 i lh bef aft nn ll ll' ;
-           found_intruse (AI_basic BI_return) H1 Hxl1 ;
-           apply in_or_app ; right ; apply in_or_app ; left ;
-           apply in_or_app ; right ; left) ;
-          try by simple_filled H1 i lh bef aft nn ll ll' ;
-          [ found_intruse (AI_basic BI_return) H1 Hxl2 ;
-            [ apply in_app_or in Hxl2 as [Habs | Habs] ;
-              [ assert (const_list ves) as Hconst ;
-                [ rewrite H3 ; apply v_to_e_is_const_list => //=
-                | intruse_among_values ves Habs Hconst ]
-              | destruct Habs as [Habs | Habs] => //=]
-            | apply in_or_app ; right ; apply in_or_app ; left ;
-              apply in_or_app ; right ; by left] 
-          | apply in_app_or in Hxl1 as [Habs | Habs] ;
-            [ assert (const_list ves) as Hconst ;
-              [ rewrite H3 ; apply v_to_e_is_const_list => //=
-              | intruse_among_values ves Habs Hconst ]
-            | destruct Habs as [Habs | Habs] => //=]].
-        { destruct H0 ;
-            (try by simple_filled H1 i lh bef aft nn ll ll' ;
-             found_intruse (AI_basic BI_return) H1 Hxl1 ;
-             apply in_or_app ; right ; apply in_or_app ; left ;
-             apply in_or_app ; right ; left) ;
-            try by simple_filled H1 i lh bef aft nn ll ll' ;
-            [ found_intruse (AI_basic BI_return) H1 Hxl2 ;
-              [ apply in_app_or in Hxl2 as [Habs | Habs] ; 
-                [ intruse_among_values vs0 Habs H0
-                | destruct Habs as [Habs | Habs] => //=]
-              | apply in_or_app ; right ; apply in_or_app ; left ;
-                apply in_or_app ; right ; by left] 
-            | apply in_app_or in Hxl1 as [Habs | Habs] ;
-              [ intruse_among_values vs0 Habs H0
-              | destruct Habs as [Habs | Habs] => //=]].
-          - simple_filled2 H1 i lh bef aft nn ll ll'.
-            found_intruse (AI_basic BI_return) H1 Hxl1 ;
-              apply in_or_app ; right ; apply in_or_app ; left ;
-                apply in_or_app ; right ; by left.
-            destruct bef ; last by inversion H1 as [[ Hhd Htl ]];
-              apply Logic.eq_sym, app_eq_nil in Htl as [_ Habs] ;
-              inversion Habs.
-            inversion H1 ; subst ; clear H1.
-            unfold lfill in Heqles ; destruct i.
-            { destruct lh0 ; last by inversion Heqles.
-              destruct (const_list l) ; inversion Heqles.
-              rewrite H2 in H0. unfold const_list in H0.
-              do 3 rewrite forallb_app in H0.
-              simpl in H0. repeat (rewrite andb_false_r in H0 + rewrite andb_false_l in H0).
-              false_assumption. }
-            fold lfill in Heqles. destruct lh0 ; first by inversion Heqles.
-            destruct (const_list l) ; last by inversion Heqles.
-            destruct (lfill _ _ _) ; inversion Heqles.
-            rewrite H2 in H0. unfold const_list in H0. rewrite forallb_app in H0.
-            simpl in H0. rewrite andb_false_r in H0. false_assumption.
-          - simple_filled2 H1 i lh bef aft nn ll ll'.
-            found_intruse (AI_basic BI_return) H1 Hxl1 ;
-              apply in_or_app ; right ; apply in_or_app ; left ;
-                apply in_or_app ; right ; by left.
-            destruct bef ; last by inversion H1 as [[ Hhd Htl ]];
-              apply Logic.eq_sym, app_eq_nil in Htl as [_ Habs] ;
-              inversion Habs.
-            inversion H1 ; subst ; clear H1.
-            unfold lfill in Heqles ; destruct i.
-            { destruct lh0 ; last by inversion Heqles.
-              destruct (const_list l) ; inversion Heqles.
-              found_intruse (AI_basic (BI_return)) H1 Hxl.
-              apply in_or_app ; right ; apply in_or_app ; left ;
-                apply in_or_app ; right ; by left. }
-            fold lfill in Heqles. destruct lh0 ; first by inversion Heqles.
-            destruct (const_list l) ; last by inversion Heqles.
-            destruct (lfill _ _ _) ; inversion Heqles.
-            found_intruse (AI_label n l0 l2) H1 Hxl1.
-          - assert (lfilled 1 (LH_rec [] n es (LH_base [] []) [])
-                            LI [AI_label n es LI]).
-            { unfold lfilled, lfill ; fold lfill => //=. by rewrite app_nil_r. }
-            destruct (lfilled_trans H3 H4) as [lh' Hfill].
-            destruct (lfilled_first_values Hfill H1) as (Habs & _ & _);
-              try done.
-          - simple_filled H1 i lh bef aft nn ll ll'.
-            found_intruse (AI_basic BI_return) H1 Hxl1.
-            rewrite Hxl1 in H0. inversion H0.
-            apply in_or_app ; right ; apply in_or_app ; left ;
-              apply in_or_app ; right ; by left.
-            rewrite Hxl1 in H0 ; inversion H0.
-          - replace [AI_trap] with ([] ++ [AI_trap])%SEQ in H2 => //=.
-            destruct (lfilled_first_values H2 H1)
-              as (Habs & _ & _) => //=. } 
-        * exfalso. eapply lfilled_return_and_reduce => //=. } 
-    - rewrite Heqes0 in H0. filled_trap H0 Hxl1. }
-  + rewrite Heqes0 in H. simple_filled H k lh bef aft nn ll ll'.
-    simpl in H. apply Logic.eq_sym, app_eq_unit in H as [[ -> Hes] | [_ Hes]].
-    apply app_eq_unit in Hes as [[ -> _ ] | [-> ->]].
-    empty_list_no_reduce.
-    unfold lfilled, lfill in H0 ; simpl in H0 ; rewrite app_nil_r in H0 ;
-      move/eqP in H0 ; subst.
-      by apply IHHred2.
-      apply app_eq_nil in Hes as [-> _ ] ; empty_list_no_reduce.
-  + (* In case Hred2 was also proved using r_local, we make use of the induction
+  destruct H ; (try by inversion Heqes0) ;
+    try by apply app_inj_tail in Heqes0 as [_ Habs] ; inversion Habs.
+  all: try by do 2 destruct vs => //.
+  all: try by do 2 destruct ves => //. 
+  - inversion Heqes0 ; subst. exfalso ; values_no_reduce.
+  - inversion Heqes0 ; subst.
+    exfalso; by eapply AI_trap_irreducible.
+  - inversion Heqes0 ; subst.
+    induction Hred1.
+    inversion H0.
+    all: subst.
+    all: try by try destruct ref; move/lfilledP in H1; inversion H1; subst;
+      lazymatch goal with
+      | H : (_)%SEQ = [_;_] |- _ =>
+          symmetry in H; try rewrite catA catA -catA in H;
+          rewrite separate1 in H;
+          apply first_values in H as (? & ? & ?);
+          try apply const_list_concat;
+          try rewrite /= const_const;
+          try rewrite /= H2
+      end.
+    all: try by move/lfilledP in H1; inversion H1; subst;
+      lazymatch goal with
+      | H : (_)%SEQ = [_;_;_] |- _ =>
+          symmetry in H; try rewrite catA catA -catA in H;
+          rewrite separate2 in H;
+          apply first_values in H as (? & ? & ?);
+          try apply const_list_concat
+      end.
+    all: try by move/lfilledP in H1; inversion H1; subst;
+      lazymatch goal with
+      | H : (_)%SEQ = [?e] |- _ =>
+          symmetry in H; try rewrite catA catA -catA in H;
+          rewrite -(app_nil_l [e]) in H;
+          apply first_values in H as (? & ? & ?);
+          try apply const_list_concat
+      end.
+    all: try by move/lfilledP in H1; inversion H1; subst;
+      lazymatch goal with
+      | H : (_)%SEQ = (_ ++ [_])%SEQ |- _ =>
+          symmetry in H; try rewrite catA catA -catA in H;
+          apply first_values in H as (? & ? & ?);
+          try apply const_list_concat;
+          subst; try apply v_to_e_is_const_list
+      end.
+    all: try by move/lfilledP in H1; inversion H1; subst;
+      lazymatch goal with
+      | H : (_)%SEQ = (_ ++ [_;_])%SEQ |- _ =>
+          symmetry in H; try rewrite catA catA -catA in H;
+          rewrite separate1 -cat_app catA in H;
+          apply first_values in H as (? & ? & ?);
+          try apply const_list_concat;
+          subst; try apply v_to_e_is_const_list
+      end.
+    all: try by move/lfilledP in H1; inversion H1; subst;
+        try (by lazymatch goal with
+      | H : (_)%SEQ = [?e] |- _ =>
+          symmetry in H; try rewrite catA catA -catA in H;
+          rewrite -(app_nil_l [e]) in H;
+          apply first_values in H as (? & ? & ?);
+          try apply const_list_concat
+                  end);
+      try (destruct bef; last (by destruct bef));
+      try (destruct vs0; last (by destruct vs0));
+      inversion H3; subst;
+      move/lfilledP in H8;
+      apply lfilled_const in H8 as [_ Habs] => //;
+      apply const_list_split in Habs as [??] => //.
+    all: try by move/lfilledP in H1; inversion H1; subst;
+      try (by lazymatch goal with
+      | H : (_)%SEQ = [?e] |- _ =>
+          symmetry in H; try rewrite catA catA -catA in H;
+          rewrite -(app_nil_l [e]) in H;
+          apply first_values in H as (? & ? & ?);
+          try apply const_list_concat
+                  end);
+      try (destruct bef; last (by destruct bef));
+      try (destruct vs0; last (by destruct vs0));
+      inversion H2; subst;
+      move/lfilledP in H7;
+      eapply filled_singleton in H7 as (_ & _ & Habs) => //;
+                                                          do 2 destruct vs => //.
+    all: try by move/lfilledP in H1; inversion H1; subst;
+      lazymatch goal with
+      | H : (_)%SEQ = [_;_;_;_] |- _ =>
+          symmetry in H; try rewrite catA catA -catA in H;
+          rewrite separate3 in H;
+          apply first_values in H as (? & ? & ?);
+          try apply const_list_concat;
+          repeat rewrite /= const_const
+      end.
+    all: try by move/lfilledP in H1; inversion H1; subst;
+      try (by lazymatch goal with
+      | H : (_)%SEQ = [?e] |- _ =>
+          symmetry in H; try rewrite catA catA -catA in H;
+          rewrite -(app_nil_l [e]) in H;
+          apply first_values in H as (? & ? & ?);
+          try apply const_list_concat
+              end);
+      destruct bef; last (by destruct bef);
+      inversion H3; subst;
+      apply hfilled_to_llfill in H0 as [llh Hllh];
+      edestruct lfilled_llfill_first_values as [??];
+      try (apply/lfilledP; exact H8);
+      try (instantiate (2 := []); exact Hllh).
+     all: try by move/lfilledP in H1; inversion H1; subst;
+      try (by lazymatch goal with
+      | H : (_)%SEQ = [?e] |- _ =>
+          symmetry in H; try rewrite catA catA -catA in H;
+          rewrite -(app_nil_l [e]) in H;
+          apply first_values in H as (? & ? & ?);
+          try apply const_list_concat
+              end);
+      destruct bef; last (by destruct bef);
+      inversion H0; subst;
+      apply hfilled_to_llfill in H4 as [llh Hllh];
+      edestruct lfilled_llfill_first_values as [??];
+      try (apply/lfilledP; exact H9);
+        try (instantiate (2 := []); exact Hllh). 
+    + move/lfilledP in H1; inversion H1; subst;
+      try (by lazymatch goal with
+      | H : (_)%SEQ = [?e] |- _ =>
+          symmetry in H; try rewrite catA catA -catA in H;
+          rewrite -(app_nil_l [e]) in H;
+          apply first_values in H as (? & ? & ?);
+          try apply const_list_concat
+              end).
+      destruct vs1; last by destruct vs1.
+      inversion H3; subst.
+      edestruct lfilled_first_values as [??].
+      exact H4. apply/lfilledP; exact H9. all: try done.
+    + edestruct lfilled_first_values as [??].
+      exact H1. instantiate (2 := []). exact H3. all: try done.
+    + move/lfilledP in H1; inversion H1; subst;
+      try (by lazymatch goal with
+      | H : (_)%SEQ = [?e] |- _ =>
+          symmetry in H; try rewrite catA catA -catA in H;
+          rewrite -(app_nil_l [e]) in H;
+          apply first_values in H as (? & ? & ?);
+          try apply const_list_concat
+              end);
+      destruct bef; last (by destruct bef);
+      inversion H2; subst.
+      apply hfilled_to_llfill in H4 as [llh Hllh];
+      edestruct lfilled_llfill_first_values as [??];
+      try (apply/lfilledP; exact H10);
+        try (instantiate (2 := []); exact Hllh).
+      all: try done.
+    + exfalso. eapply lfilled_return_and_reduce => //=.
+  - rewrite Heqes0 in H0.
+    move/lfilledP in H0; inversion H0.
+    all: try by do 2 destruct vs => //.
+    all: by do 2 destruct bef => //.
+  - rewrite Heqes0 in H.
+    move/lfilledP in H; inversion H; subst.
+    all: try by do 2 destruct bef => //.
+    all: try by do 2 destruct vs => //.
+    destruct vs; last by destruct vs, es0 => //; empty_list_no_reduce.
+    destruct es0; first by empty_list_no_reduce.
+    inversion H1; subst.
+    destruct es0, es'1 => //.
+    move/lfilledP in H0; inversion H0; subst.
+    simpl in *.
+    rewrite cats0.
+    apply IHHred2 => //. 
+  - (* In case Hred2 was also proved using r_local, we make use of the induction
          hypothesis IHnnn *)
     inversion Heqes0 ; subst. clear IHHred2.
     assert (length_rec es < nnn).
