theories/iris/helpers/reduce_det/reduce_det_return.v
@@ -2,6 +2,8 @@ From mathcomp Require Import ssreflect eqtype seq ssrbool.
 From stdpp Require Import base list.
 From Wasm.iris.helpers.prelude Require Export iris_reduce_det_prelude.
 
+Set Bullet Behavior "Strict Subproofs".
+
 Lemma return_det vs n i lh s f f0 es s' f' es' :
   const_list vs ->
   length vs = n ->
@@ -15,137 +17,42 @@ Proof.
          and thus all the work must be performed by hand *)
   left ; remember [AI_local n f0 es] as es0.
   rewrite <- app_nil_l in Heqes0.
-  induction Hred ; try by inversion Heqes0 ;
-    try by apply app_inj_tail in Heqes0 as [_ Habs] ; inversion Habs.
-  { destruct H2 ; try by inversion Heqes0 ;
-      try by apply app_inj_tail in Heqes0 as [_ Habs] ; inversion Habs.
-    - inversion Heqes0 ; subst.
-      destruct i ; unfold lfilled, lfill in H1.
-      { destruct lh ; last by false_assumption.
-        destruct (const_list l) ; last by false_assumption.
-        move/eqP in H1. rewrite H1 in H2.
-        unfold const_list in H2 ; do 3 rewrite forallb_app in H2.
-        apply andb_true_iff in H2 as [_ Habs].
-        apply andb_true_iff in Habs as [Habs _].
-        apply andb_true_iff in Habs as [_ Habs].
-        apply andb_true_iff in Habs as [Habs _].
-        inversion Habs. }
-      fold lfill in H1. destruct lh ; first by false_assumption.
-      destruct (const_list l) ; last by false_assumption.
-      destruct (lfill _ _ _) ; last by false_assumption.
-      move/eqP in H1. rewrite H1 in H2. unfold const_list in H2.
-      rewrite forallb_app in H2. apply andb_true_iff in H2 as [_ Habs].
-      simpl in Habs. false_assumption.
-    - inversion Heqes0. rewrite <- H5 in H1.
-      destruct i ; unfold lfilled, lfill in H1.
-      { destruct lh ; last by false_assumption.
-        destruct (const_list l) ; last by false_assumption. move/eqP in H1.
-        found_intruse (AI_basic BI_return) H1 Hxl1.
-        apply in_or_app ; right. apply in_or_app ; left.
-        apply in_or_app ; right. by left. }
-      fold lfill in H1. destruct lh ; first by false_assumption.
-      destruct (const_list l) ; last by false_assumption.
-      destruct (lfill _ _ _) ; last by false_assumption.
-      move/eqP in H1. found_intruse (AI_label n1 l0 l2) H1 Hxl1.
-    - inversion Heqes0 ; subst.
-      destruct (lfilled_first_values H1 H4) as (_ & _ & Hvs) => //=.
-      destruct (Hvs (Logic.eq_sym H6)) as [Hrew _].
-        by rewrite Hrew.
-    - rewrite Heqes0 in H3. filled_trap H3 Hxl1. }
-  + rewrite Heqes0 in H2. simple_filled H2 k lh0 bef aft nn ll ll'.
-    simpl in H2. apply Logic.eq_sym, app_eq_unit in H2 as [[-> Hes] | [_ Hes]].
-    apply app_eq_unit in Hes as [[-> _]|[Hes ->]].
-    empty_list_no_reduce.
-    unfold lfilled, lfill in H3. simpl in H3. move/eqP in H3.
-    rewrite app_nil_r in H3. subst. apply IHHred => //=.
-    apply app_eq_nil in Hes as [-> _] ; empty_list_no_reduce.
-  + { inversion Heqes0 ; subst.
-      induction Hred ;
-        (try by simple_filled H1 i lh bef aft nn ll ll' ;
-         found_intruse (AI_basic BI_return) H1 Hxl1 ;
-         apply in_or_app ; right ; apply in_or_app ; left ;
-         apply in_or_app ; right ; left) ;
-        try by simple_filled H1 i lh bef aft nn ll ll' ;
-        [ found_intruse (AI_basic BI_return) H1 Hxl2 ;
-          [ apply in_app_or in Hxl2 as [Habs | Habs] ;
-            [ assert (const_list ves) as Hconst ;
-              [ rewrite H3 ; apply v_to_e_is_const_list => //=
-              | intruse_among_values ves Habs Hconst ]
-            | destruct Habs as [Habs | Habs] => //=]
-          | apply in_or_app ; right ; apply in_or_app ; left ;
-            apply in_or_app ; right ; by left] 
-        | apply in_app_or in Hxl1 as [Habs | Habs] ;
-          [ assert (const_list ves) as Hconst ;
-            [ rewrite H3 ; apply v_to_e_is_const_list => //=
-            | intruse_among_values ves Habs Hconst ]
-          | destruct Habs as [Habs | Habs] => //=]].
-      { destruct H0 ;
-          (try by simple_filled H1 i lh bef aft nn ll ll' ;
-           found_intruse (AI_basic BI_return) H1 Hxl1 ;
-           apply in_or_app ; right ; apply in_or_app ; left ;
-           apply in_or_app ; right ; left) ;
-          try by simple_filled H1 i lh bef aft nn ll ll' ;
-          [ found_intruse (AI_basic BI_return) H1 Hxl2 ;
-            [ apply in_app_or in Hxl2 as [Habs | Habs] ; 
-              [ intruse_among_values vs0 Habs H0
-              | destruct Habs as [Habs | Habs] => //=]
-            | apply in_or_app ; right ; apply in_or_app ; left ;
-              apply in_or_app ; right ; by left] 
-          | apply in_app_or in Hxl1 as [Habs | Habs] ;
-            [ intruse_among_values vs0 Habs H0
-            | destruct Habs as [Habs | Habs] => //=]].
-        - simple_filled2 H1 i lh bef aft nn ll ll'.
-          found_intruse (AI_basic BI_return) H1 Hxl1 ;
-            apply in_or_app ; right ; apply in_or_app ; left ;
-              apply in_or_app ; right ; by left.
-          destruct bef ; last by inversion H1 as [[ Hhd Htl ]];
-            apply Logic.eq_sym, app_eq_nil in Htl as [_ Habs] ;
-            inversion Habs.
-          inversion H1 ; subst ; clear H1.
-          unfold lfill in Heqles ; destruct i.
-          { destruct lh0 ; last by inversion Heqles.
-            destruct (const_list l) ; inversion Heqles.
-            rewrite H2 in H0. unfold const_list in H0.
-            do 3 rewrite forallb_app in H0.
-            simpl in H0. repeat (rewrite andb_false_r in H0 + rewrite andb_false_l in H0).
-            false_assumption. }
-          fold lfill in Heqles. destruct lh0 ; first by inversion Heqles.
-          destruct (const_list l) ; last by inversion Heqles.
-          destruct (lfill _ _ _) ; inversion Heqles.
-          rewrite H2 in H0. unfold const_list in H0. rewrite forallb_app in H0.
-          simpl in H0. rewrite andb_false_r in H0. false_assumption.
-        - simple_filled2 H1 i lh bef aft nn ll ll'.
-          found_intruse (AI_basic BI_return) H1 Hxl1 ;
-            apply in_or_app ; right ; apply in_or_app ; left ;
-              apply in_or_app ; right ; by left.
-          destruct bef ; last by inversion H1 as [[ Hhd Htl ]];
-            apply Logic.eq_sym, app_eq_nil in Htl as [_ Habs] ;
-            inversion Habs.
-          inversion H1 ; subst ; clear H1.
-          unfold lfill in Heqles ; destruct i.
-          { destruct lh0 ; last by inversion Heqles.
-            destruct (const_list l) ; inversion Heqles.
-            found_intruse (AI_basic (BI_return)) H1 Hxl1.
-            apply in_or_app ; right ; apply in_or_app ; left ;
-              apply in_or_app ; right ; by left. }
-          fold lfill in Heqles. destruct lh0 ; first by inversion Heqles.
-          destruct (const_list l) ; last by inversion Heqles.
-          destruct (lfill _ _ _) ; inversion Heqles.
-          found_intruse (AI_label n l0 l2) H1 Hxl1.
-        - assert (lfilled 1 (LH_rec [] n es (LH_base [] []) [])
-                          LI [AI_label n es LI]).
-          { unfold lfilled, lfill ; fold lfill => //=. by rewrite app_nil_r. }
-          destruct (lfilled_trans H3 H4) as [lh' Hfill].
-          destruct (lfilled_first_values Hfill H1) as (Habs & _ & _);
-            try done.
-        - simple_filled H1 i lh bef aft nn ll ll'.
-          found_intruse (AI_basic BI_return) H1 Hxl1.
-          rewrite Hxl1 in H0. inversion H0.
-          apply in_or_app ; right ; apply in_or_app ; left ;
-            apply in_or_app ; right ; by left.
-          rewrite Hxl1 in H0 ; inversion H0.
-        - replace [AI_trap] with ([] ++ [AI_trap])%SEQ in H2 => //=.
-          destruct (lfilled_first_values H2 H1)
-            as (Habs & _ & _) => //=. } 
-      * exfalso. eapply lfilled_return_and_reduce => //=. }
+  induction Hred.
+  inversion H2.
+  all: remember Heqes0 as Heqes; clear HeqHeqes Heqes0; subst.
+  all: try done.
+  all: try by do 2 destruct vs0 => //.
+  all: try by do 2 destruct vcs => //. 
+  - inversion Heqes; subst.
+    apply lfilled_const in H1 as [??] => //.
+    apply const_list_split in H1 as [??] => //.
+  - inversion Heqes; subst.
+    apply filled_singleton in H1 as (? & ? & ?) => //.
+    all: do 2 destruct vs => //.
+  - inversion Heqes; subst.
+    edestruct lfilled_first_values as (_ & _ & Hsol).
+    exact H5. exact H1. all: try done.
+    apply Hsol in H4 as [-> ->] => //.
+  - move/lfilledP in H4; inversion H4; subst.
+    do 2 destruct vs0 => //.
+    all: do 2 destruct bef => //.
+  - move/lfilledP in H2; inversion H2; subst.
+    all: move/lfilledP in H3; inversion H3; subst.
+    all: try by do 2 destruct vs0 => //.
+    all: try by do 2 destruct bef => //.
+    destruct vs0; last by destruct vs0, es0 => //; empty_list_no_reduce.
+    destruct es0; first empty_list_no_reduce.
+    inversion H0; subst.
+    destruct es0, es'0 => //.
+    rewrite /= cats0.
+    by apply IHHred.
+  - inversion Heqes; subst.
+    exfalso; eapply lfilled_return_and_reduce.
+    exact Hred.
+    2: exact H1.
+    done.
+    instantiate (1 := LH_base [] []).
+    instantiate (1 := 0).
+    unfold lfilled, lfill => //=.
+    rewrite app_nil_r => //.
 Qed.
