theories/iris/helpers/reduce_det/reduce_det_select.v
@@ -2,15 +2,259 @@ From mathcomp Require Import ssreflect eqtype seq ssrbool.
 From stdpp Require Import base list.
 From Wasm.iris.helpers.prelude Require Export iris_reduce_det_prelude.
 
+Set Bullet Behavior "Strict Subproofs".
+
 Lemma select_false_det v1 v2 n s f s' f' es:
   n = Wasm_int.int_zero i32m ->
-  reduce s f [AI_basic (BI_const v1); AI_basic (BI_const v2); AI_basic (BI_const (VAL_int32 n)); AI_basic BI_select] s' f' es ->
-  reduce_det_goal s f [AI_basic (BI_const v2)] s' f' es [AI_basic (BI_const v1); AI_basic (BI_const v2); AI_basic (BI_const (VAL_int32 n)); AI_basic BI_select].
+  reduce s f [AI_const v1; AI_const v2; AI_basic (BI_const (VAL_int32 n)); AI_basic BI_select] s' f' es ->
+  reduce_det_goal s f [AI_const v2] s' f' es [AI_const v1; AI_const v2; AI_basic (BI_const (VAL_int32 n)); AI_basic BI_select].
 Proof.
   move => H Hred.
-  only_one [AI_basic (BI_const v1) ; AI_basic (BI_const v2);
-            AI_basic (BI_const (VAL_int32 n)) ; AI_basic BI_select] Hred ;
-    [done | by inversion Heqes ; subst ].
+    
+  let Hfill := fresh "Hfill" in
+  let Hfill' := fresh "Hfill" in
+  let IHHred := fresh "IHHred" in
+    lazymatch goal with
+      Hred : reduce _ _ ?es _ _ _ |- _ =>
+      remember es as esnew eqn:Heqesnew;
+      induction Hred as [? ? ? ? Hred | | | | | | | | | | | | | | | | | | | | | | | | | | | | | | | | | | | | | | | | | ?? esnewest ??????? Hred IHHred Hfill Hfill' | ];
+      first destruct Hred as [| | | | | | | | | | | | | | | | | | | | | | | | | | | | | | | | | | | | | | | | | | ??? Hfill];
+      try (by inversion Heqesnew) ;
+      try (by lazymatch goal with
+                _ : (v_to_e_list ?vs ++ _)%SEQ = _ |- _ => do 5 destruct vs => //
+              end);
+      try (by lazymatch goal with
+                _ : (?vs ++ _)%SEQ = _ |- _ => do 5 destruct vs => //
+              end);
+      try (by inversion Heqesnew; subst; left);
+      try (move/lfilledP in Hfill; inversion Hfill; subst;
+            try (by lazymatch goal with
+                _ : (?vs ++ _)%SEQ = _ |- _ => do 5 (destruct vs => //; try by destruct v1, v2; try destruct v; try destruct v0)
+                    end))  ;
+      last (move/lfilledP in Hfill'; inversion Hfill'; subst ;
+      lazymatch goal with
+        _ : (?vs ++ ?esnewest ++ ?es'0)%SEQ = _ |- _ =>
+          destruct vs;
+          first (
+              destruct es'0 ;
+              [ repeat rewrite cats0 /=;
+                  lazymatch goal with H : ([] ++ _ ++ [])%SEQ = _ |- _ => rewrite cats0 /= in H; subst end;
+                try apply IHHred => //
+              | lazymatch goal with
+                  H : ([] ++ _ ++ _ :: _)%SEQ = _ |- _ =>
+                    do 4 try (destruct esnewest; first by inversion H; subst;
+                              apply values_no_reduce in Hred; repeat rewrite /= const_const);
+                    try (destruct esnewest; last by inversion H);
+                    inversion H
+                end] ) 
+      end)
+    end.
+  inversion H4; subst.
+  destruct vs.
+  - destruct esnewest; first empty_list_no_reduce.
+    inversion H3; subst.
+    destruct esnewest; first by apply values_no_reduce in Hred; try rewrite /= const_const.
+    inversion H5; subst.
+    destruct esnewest; first by apply values_no_reduce in Hred; repeat rewrite /= const_const.
+    inversion H6; subst. destruct esnewest, es'0 => //.
+    clear -Hred.
+      lazymatch goal with
+    | _ : reduce _ _ ?esn _ _ _ |- _ => remember esn as ves
+    end.
+    exfalso. 
+    induction Hred as [? ? ? ? H02 | | | | | | | | | | | | | | | | | | | | | | | | | | | | | | | | | | | | | | | | | ???????????? H02 H03 | ];
+        first destruct H02 as [| | | | | | | | | | | | | | | | | | | | | | | | | | | | | | | | | | | | | | | | | | ??? H01 ]; 
+        try (by inversion Heqves);
+        try (by do 5 destruct vs => //);
+      try (by do 5 destruct ves => //);
+        [ by move/lfilledP in H01; inversion H01; subst;
+          try (by do 4 (destruct vs => //; try by destruct v2; try destruct v));
+          do 4 (destruct bef => //; try by destruct v2; try destruct v)
+        | move/lfilledP in H02; inversion H02; subst;
+          try (by do 4 (destruct vs => //; try by destruct v2; try destruct v));
+          try (by do 4 (destruct bef => //; try by destruct v2; try destruct v)) ;
+          destruct vs;
+          first (
+              do 4 try (destruct es; first by inversion H3; subst; apply values_no_reduce in Hred; repeat rewrite /= const_const);
+              inversion H3; subst;
+              destruct es => //; apply IHHred => //
+              )
+        ].
+    inversion H3; subst.
+    destruct vs.
+    + destruct es; first empty_list_no_reduce.
+      inversion H2; subst.
+      destruct es; first by apply values_no_reduce in Hred.
+      inversion H4; subst. destruct es, es'0 => //.
+      clear -Hred.
+      lazymatch goal with
+    | _ : reduce _ _ ?esn _ _ _ |- _ => remember esn as ves
+    end.
+    exfalso. 
+    induction Hred as [? ? ? ? H02 | | | | | | | | | | | | | | | | | | | | | | | | | | | | | | | | | | | | | | | | | ???????????? H02 H03 | ];
+        first destruct H02 as [| | | | | | | | | | | | | | | | | | | | | | | | | | | | | | | | | | | | | | | | | | ??? H01 ]; 
+        try (by inversion Heqves);
+        try (by destruct vs; try destruct vs; try destruct vs; try destruct vs; inversion Heqves);
+        try (by destruct ves; try destruct ves; try destruct ves; try destruct ves; inversion Heqves);
+        [ by move/lfilledP in H01; inversion H01; subst;
+          try (by do 4 destruct vs => //);
+          do 4 destruct bef => //
+        | move/lfilledP in H02; inversion H02; subst;
+          try (by do 4 destruct vs => //);
+          try (by do 4 destruct bef => //);
+          destruct vs;
+          first (
+              do 4 try (destruct es; first by inversion H3; subst; apply values_no_reduce in Hred);
+              inversion H3; subst;
+              destruct es => //; apply IHHred => //
+              )
+        ].
+    inversion H3; subst. 
+    destruct vs; last by inversion H2; subst.
+    destruct es; first empty_list_no_reduce.
+    inversion H2; subst.
+    destruct es, es'0 => //.
+    clear - Hred.
+    lazymatch goal with
+    | _ : reduce _ _ ?esn _ _ _ |- _ => remember esn as ves
+    end.
+    induction Hred as [? ? ? ? H02 | | | | | | | | | | | | | | | | | | | | | | | | | | | | | | | | | | | | | | | | | ???????????? H02 H03 | ];
+        first destruct H02 as [| | | | | | | | | | | | | | | | | | | | | | | | | | | | | | | | | | | | | | | | | | ??? H01 ]; 
+        try (by inversion Heqves);
+        try (by destruct vs; try destruct vs; try destruct vs; try destruct vs; inversion Heqves);
+        try (by destruct ves; try destruct ves; try destruct ves; try destruct ves; inversion Heqves);
+        [ by move/lfilledP in H01; inversion H01; subst;
+          try (by do 4 destruct vs => //);
+          do 4 destruct bef => //
+        | move/lfilledP in H02; inversion H02; subst;
+          try (by do 4 destruct vs => //);
+          try (by do 4 destruct bef => //) ;
+          destruct vs;
+          first (
+              do 4 try (destruct es; first by inversion H3; subst; apply values_no_reduce in Hred);
+              inversion H3; subst; 
+              destruct es => //; apply IHHred => //
+              )
+        ].
+    inversion H3; subst. destruct vs, es, es'0 => //.
+    + destruct vs.
+      2:{ inversion H2; subst. simpl in H. destruct v2; try destruct v => //. }   inversion H2; subst.
+      destruct es; first empty_list_no_reduce.
+      inversion H4; subst.
+      destruct es => //.
+      clear - Hred.
+      exfalso.
+      lazymatch goal with
+    | _ : reduce _ _ ?esn _ _ _ |- _ => remember esn as ves
+    end.
+    induction Hred as [? ? ? ? H02 | | | | | | | | | | | | | | | | | | | | | | | | | | | | | | | | | | | | | | | | | ???????????? H02 H03 | ];
+        first destruct H02 as [| | | | | | | | | | | | | | | | | | | | | | | | | | | | | | | | | | | | | | | | | | ??? H01 ]; 
+        try (by inversion Heqves);
+        try (by destruct vs; try destruct vs; try destruct vs; try destruct vs; inversion Heqves);
+        try (by destruct ves; try destruct ves; try destruct ves; try destruct ves; inversion Heqves);
+        [ by move/lfilledP in H01; inversion H01; subst;
+          try (by do 4 destruct vs => //);
+          do 4 destruct bef => //
+        | move/lfilledP in H02; inversion H02; subst;
+          try (by do 4 destruct vs => //);
+          try (by do 4 destruct bef => //) ;
+          destruct vs;
+          first (
+              do 4 try (destruct es; first by inversion H3; subst; apply values_no_reduce in Hred);
+              inversion H3; subst; 
+              destruct es => //; apply IHHred => //
+              )
+        ].
+    inversion H3; subst.
+    done.
+  - inversion H3; subst.
+     destruct vs.
+    + destruct esnewest; first empty_list_no_reduce.
+      inversion H5; subst.
+      destruct esnewest; first by apply values_no_reduce in Hred.
+      inversion H6; subst. destruct esnewest, es'0 => //.
+      clear -Hred.
+      lazymatch goal with
+    | _ : reduce _ _ ?esn _ _ _ |- _ => remember esn as ves
+    end.
+    exfalso. 
+    induction Hred as [? ? ? ? H02 | | | | | | | | | | | | | | | | | | | | | | | | | | | | | | | | | | | | | | | | | ???????????? H02 H03 | ];
+        first destruct H02 as [| | | | | | | | | | | | | | | | | | | | | | | | | | | | | | | | | | | | | | | | | | ??? H01 ]; 
+        try (by inversion Heqves);
+        try (by destruct vs; try destruct vs; try destruct vs; try destruct vs; inversion Heqves);
+        try (by destruct ves; try destruct ves; try destruct ves; try destruct ves; inversion Heqves);
+        [ by move/lfilledP in H01; inversion H01; subst;
+          try (by do 4 destruct vs => //);
+          do 4 destruct bef => //
+        | move/lfilledP in H02; inversion H02; subst;
+          try (by do 4 destruct vs => //);
+          try (by do 4 destruct bef => //);
+          destruct vs;
+          first (
+              do 4 try (destruct es; first by inversion H3; subst; apply values_no_reduce in Hred);
+              inversion H3; subst;
+              destruct es => //; apply IHHred => //
+              )
+        ].
+    inversion H3; subst. 
+    destruct vs; last by inversion H2; subst.
+    destruct es; first empty_list_no_reduce.
+    inversion H2; subst.
+    destruct es, es'0 => //.
+    clear - Hred.
+    lazymatch goal with
+    | _ : reduce _ _ ?esn _ _ _ |- _ => remember esn as ves
+    end.
+    induction Hred as [? ? ? ? H02 | | | | | | | | | | | | | | | | | | | | | | | | | | | | | | | | | | | | | | | | | ???????????? H02 H03 | ];
+        first destruct H02 as [| | | | | | | | | | | | | | | | | | | | | | | | | | | | | | | | | | | | | | | | | | ??? H01 ]; 
+        try (by inversion Heqves);
+        try (by destruct vs; try destruct vs; try destruct vs; try destruct vs; inversion Heqves);
+        try (by destruct ves; try destruct ves; try destruct ves; try destruct ves; inversion Heqves);
+        [ by move/lfilledP in H01; inversion H01; subst;
+          try (by do 4 destruct vs => //);
+          do 4 destruct bef => //
+        | move/lfilledP in H02; inversion H02; subst;
+          try (by do 4 destruct vs => //);
+          try (by do 4 destruct bef => //) ;
+          destruct vs;
+          first (
+              do 4 try (destruct es; first by inversion H3; subst; apply values_no_reduce in Hred);
+              inversion H3; subst; 
+              destruct es => //; apply IHHred => //
+              )
+        ].
+    inversion H3; subst. destruct vs, es, es'0 => //.
+    + destruct vs.
+      2:{ inversion H5; subst. simpl in H0. repeat rewrite const_const in H0. done. }
+      inversion H5; subst.
+      destruct esnewest; first empty_list_no_reduce.
+      inversion H6; subst.
+      destruct esnewest => //.
+      clear - Hred.
+      exfalso.
+      lazymatch goal with
+    | _ : reduce _ _ ?esn _ _ _ |- _ => remember esn as ves
+    end.
+    induction Hred as [? ? ? ? H02 | | | | | | | | | | | | | | | | | | | | | | | | | | | | | | | | | | | | | | | | | ???????????? H02 H03 | ];
+        first destruct H02 as [| | | | | | | | | | | | | | | | | | | | | | | | | | | | | | | | | | | | | | | | | | ??? H01 ]; 
+        try (by inversion Heqves);
+        try (by destruct vs; try destruct vs; try destruct vs; try destruct vs; inversion Heqves);
+        try (by destruct ves; try destruct ves; try destruct ves; try destruct ves; inversion Heqves);
+        [ by move/lfilledP in H01; inversion H01; subst;
+          try (by do 4 destruct vs => //);
+          do 4 destruct bef => //
+        | move/lfilledP in H02; inversion H02; subst;
+          try (by do 4 destruct vs => //);
+          try (by do 4 destruct bef => //) ;
+          destruct vs;
+          first (
+              do 4 try (destruct es; first by inversion H3; subst; apply values_no_reduce in Hred);
+              inversion H3; subst; 
+              destruct es => //; apply IHHred => //
+              )
+        ].
+    inversion H3; subst.
+    done.
 Qed.
 
 Lemma select_true_det v1 v2 n s f s' f' es:
@@ -19,7 +263,250 @@ Lemma select_true_det v1 v2 n s f s' f' es:
   reduce_det_goal s f [AI_basic (BI_const v1)] s' f' es [AI_basic (BI_const v1); AI_basic (BI_const v2); AI_basic (BI_const (VAL_int32 n)); AI_basic BI_select].
 Proof.
   move => H Hred.
-  only_one [AI_basic (BI_const v1) ; AI_basic (BI_const v2);
-            AI_basic (BI_const (VAL_int32 n)) ; AI_basic BI_select] Hred ;
-    [ by inversion Heqes ; subst | done ].
+    
+  let Hfill := fresh "Hfill" in
+  let Hfill' := fresh "Hfill" in
+  let IHHred := fresh "IHHred" in
+    lazymatch goal with
+      Hred : reduce _ _ ?es _ _ _ |- _ =>
+      remember es as esnew eqn:Heqesnew;
+      induction Hred as [? ? ? ? Hred | | | | | | | | | | | | | | | | | | | | | | | | | | | | | | | | | | | | | | | | | ?? esnewest ??????? Hred IHHred Hfill Hfill' | ];
+      first destruct Hred as [| | | | | | | | | | | | | | | | | | | | | | | | | | | | | | | | | | | | | | | | | | ??? Hfill];
+      try (by inversion Heqesnew) ;
+      try (by lazymatch goal with
+                _ : (v_to_e_list ?vs ++ _)%SEQ = _ |- _ => do 5 destruct vs => //
+              end);
+      try (by lazymatch goal with
+                _ : (?vs ++ _)%SEQ = _ |- _ => do 5 destruct vs => //
+              end);
+      try (by inversion Heqesnew; subst; left);
+      try (move/lfilledP in Hfill; inversion Hfill; subst;
+            try (by lazymatch goal with
+                _ : (?vs ++ _)%SEQ = _ |- _ => do 5 (destruct vs => //; try by destruct v1, v2; try destruct v; try destruct v0)
+                    end))  ;
+      last (move/lfilledP in Hfill'; inversion Hfill'; subst ;
+      lazymatch goal with
+        _ : (?vs ++ ?esnewest ++ ?es'0)%SEQ = _ |- _ =>
+          destruct vs;
+          first (
+              destruct es'0 ;
+              [ repeat rewrite cats0 /=;
+                  lazymatch goal with H : ([] ++ _ ++ [])%SEQ = _ |- _ => rewrite cats0 /= in H; subst end;
+                try apply IHHred => //
+              | lazymatch goal with
+                  H : ([] ++ _ ++ _ :: _)%SEQ = _ |- _ =>
+                    do 4 try (destruct esnewest; first by inversion H; subst;
+                              apply values_no_reduce in Hred; repeat rewrite /= const_const);
+                    try (destruct esnewest; last by inversion H);
+                    inversion H
+                end] ) 
+      end)
+    end.
+  inversion H4; subst.
+  destruct vs.
+  - destruct esnewest; first empty_list_no_reduce.
+    inversion H5; subst.
+    destruct esnewest; first by apply values_no_reduce in Hred; try rewrite /= const_const.
+    inversion H6; subst.
+    destruct esnewest; first by apply values_no_reduce in Hred; repeat rewrite /= const_const.
+    inversion H7; subst. destruct esnewest, es'0 => //.
+    clear -Hred.
+      lazymatch goal with
+    | _ : reduce _ _ ?esn _ _ _ |- _ => remember esn as ves
+    end.
+    exfalso. 
+    induction Hred as [? ? ? ? H02 | | | | | | | | | | | | | | | | | | | | | | | | | | | | | | | | | | | | | | | | | ???????????? H02 H03 | ];
+        first destruct H02 as [| | | | | | | | | | | | | | | | | | | | | | | | | | | | | | | | | | | | | | | | | | ??? H01 ]; 
+        try (by inversion Heqves);
+        try (by do 5 destruct vs => //);
+      try (by do 5 destruct ves => //);
+        [ by move/lfilledP in H01; inversion H01; subst;
+          try (by do 4 (destruct vs => //; try by destruct v2; try destruct v));
+          do 4 (destruct bef => //; try by destruct v2; try destruct v)
+        | move/lfilledP in H02; inversion H02; subst;
+          try (by do 4 (destruct vs => //; try by destruct v2; try destruct v));
+          try (by do 4 (destruct bef => //; try by destruct v2; try destruct v)) ;
+          destruct vs;
+          first (
+              do 4 try (destruct es; first by inversion H3; subst; apply values_no_reduce in Hred; repeat rewrite /= const_const);
+              inversion H3; subst;
+              destruct es => //; apply IHHred => //
+              )
+        ].
+    inversion H3; subst.
+    destruct vs.
+    + destruct es; first empty_list_no_reduce.
+      inversion H2; subst.
+      destruct es; first by apply values_no_reduce in Hred.
+      inversion H4; subst. destruct es, es'0 => //.
+      clear -Hred.
+      lazymatch goal with
+    | _ : reduce _ _ ?esn _ _ _ |- _ => remember esn as ves
+    end.
+    exfalso. 
+    induction Hred as [? ? ? ? H02 | | | | | | | | | | | | | | | | | | | | | | | | | | | | | | | | | | | | | | | | | ???????????? H02 H03 | ];
+        first destruct H02 as [| | | | | | | | | | | | | | | | | | | | | | | | | | | | | | | | | | | | | | | | | | ??? H01 ]; 
+        try (by inversion Heqves);
+        try (by destruct vs; try destruct vs; try destruct vs; try destruct vs; inversion Heqves);
+        try (by destruct ves; try destruct ves; try destruct ves; try destruct ves; inversion Heqves);
+        [ by move/lfilledP in H01; inversion H01; subst;
+          try (by do 4 destruct vs => //);
+          do 4 destruct bef => //
+        | move/lfilledP in H02; inversion H02; subst;
+          try (by do 4 destruct vs => //);
+          try (by do 4 destruct bef => //);
+          destruct vs;
+          first (
+              do 4 try (destruct es; first by inversion H3; subst; apply values_no_reduce in Hred);
+              inversion H3; subst;
+              destruct es => //; apply IHHred => //
+              )
+        ].
+    inversion H3; subst. 
+    destruct vs; last by inversion H2; subst.
+    destruct es; first empty_list_no_reduce.
+    inversion H2; subst.
+    destruct es, es'0 => //.
+    clear - Hred.
+    lazymatch goal with
+    | _ : reduce _ _ ?esn _ _ _ |- _ => remember esn as ves
+    end.
+    induction Hred as [? ? ? ? H02 | | | | | | | | | | | | | | | | | | | | | | | | | | | | | | | | | | | | | | | | | ???????????? H02 H03 | ];
+        first destruct H02 as [| | | | | | | | | | | | | | | | | | | | | | | | | | | | | | | | | | | | | | | | | | ??? H01 ]; 
+        try (by inversion Heqves);
+        try (by destruct vs; try destruct vs; try destruct vs; try destruct vs; inversion Heqves);
+        try (by destruct ves; try destruct ves; try destruct ves; try destruct ves; inversion Heqves);
+        [ by move/lfilledP in H01; inversion H01; subst;
+          try (by do 4 destruct vs => //);
+          do 4 destruct bef => //
+        | move/lfilledP in H02; inversion H02; subst;
+          try (by do 4 destruct vs => //);
+          try (by do 4 destruct bef => //) ;
+          destruct vs;
+          first (
+              do 4 try (destruct es; first by inversion H3; subst; apply values_no_reduce in Hred);
+              inversion H3; subst; 
+              destruct es => //; apply IHHred => //
+              )
+        ].
+    inversion H3; subst. destruct vs, es, es'0 => //.
+    + destruct vs.
+      2:{ inversion H2; subst. simpl in H. done. }
+      destruct es; first empty_list_no_reduce.
+      inversion H2; subst.
+      destruct es => //.
+      clear - Hred.
+      exfalso.
+      lazymatch goal with
+    | _ : reduce _ _ ?esn _ _ _ |- _ => remember esn as ves
+    end.
+    induction Hred as [? ? ? ? H02 | | | | | | | | | | | | | | | | | | | | | | | | | | | | | | | | | | | | | | | | | ???????????? H02 H03 | ];
+        first destruct H02 as [| | | | | | | | | | | | | | | | | | | | | | | | | | | | | | | | | | | | | | | | | | ??? H01 ]; 
+        try (by inversion Heqves);
+        try (by destruct vs; try destruct vs; try destruct vs; try destruct vs; inversion Heqves);
+        try (by destruct ves; try destruct ves; try destruct ves; try destruct ves; inversion Heqves);
+        [ by move/lfilledP in H01; inversion H01; subst;
+          try (by do 4 destruct vs => //);
+          do 4 destruct bef => //
+        | move/lfilledP in H02; inversion H02; subst;
+          try (by do 4 destruct vs => //);
+          try (by do 4 destruct bef => //) ;
+          destruct vs;
+          first (
+              do 4 try (destruct es; first by inversion H3; subst; apply values_no_reduce in Hred);
+              inversion H3; subst; 
+              destruct es => //; apply IHHred => //
+              )
+        ].
+    inversion H3; subst.
+    done.
+  - inversion H3; subst.
+     destruct vs.
+    + destruct esnewest; first empty_list_no_reduce.
+      inversion H5; subst.
+      destruct esnewest; first by apply values_no_reduce in Hred.
+      inversion H8; subst. destruct esnewest, es'0 => //.
+      clear -Hred.
+      lazymatch goal with
+    | _ : reduce _ _ ?esn _ _ _ |- _ => remember esn as ves
+    end.
+    exfalso. 
+    induction Hred as [? ? ? ? H02 | | | | | | | | | | | | | | | | | | | | | | | | | | | | | | | | | | | | | | | | | ???????????? H02 H03 | ];
+        first destruct H02 as [| | | | | | | | | | | | | | | | | | | | | | | | | | | | | | | | | | | | | | | | | | ??? H01 ]; 
+        try (by inversion Heqves);
+        try (by destruct vs; try destruct vs; try destruct vs; try destruct vs; inversion Heqves);
+        try (by destruct ves; try destruct ves; try destruct ves; try destruct ves; inversion Heqves);
+        [ by move/lfilledP in H01; inversion H01; subst;
+          try (by do 4 destruct vs => //);
+          do 4 destruct bef => //
+        | move/lfilledP in H02; inversion H02; subst;
+          try (by do 4 destruct vs => //);
+          try (by do 4 destruct bef => //);
+          destruct vs;
+          first (
+              do 4 try (destruct es; first by inversion H3; subst; apply values_no_reduce in Hred);
+              inversion H3; subst;
+              destruct es => //; apply IHHred => //
+              )
+        ].
+    inversion H3; subst. 
+    destruct vs; last by inversion H2; subst.
+    destruct es; first empty_list_no_reduce.
+    inversion H2; subst.
+    destruct es, es'0 => //.
+    clear - Hred.
+    lazymatch goal with
+    | _ : reduce _ _ ?esn _ _ _ |- _ => remember esn as ves
+    end.
+    induction Hred as [? ? ? ? H02 | | | | | | | | | | | | | | | | | | | | | | | | | | | | | | | | | | | | | | | | | ???????????? H02 H03 | ];
+        first destruct H02 as [| | | | | | | | | | | | | | | | | | | | | | | | | | | | | | | | | | | | | | | | | | ??? H01 ]; 
+        try (by inversion Heqves);
+        try (by destruct vs; try destruct vs; try destruct vs; try destruct vs; inversion Heqves);
+        try (by destruct ves; try destruct ves; try destruct ves; try destruct ves; inversion Heqves);
+        [ by move/lfilledP in H01; inversion H01; subst;
+          try (by do 4 destruct vs => //);
+          do 4 destruct bef => //
+        | move/lfilledP in H02; inversion H02; subst;
+          try (by do 4 destruct vs => //);
+          try (by do 4 destruct bef => //) ;
+          destruct vs;
+          first (
+              do 4 try (destruct es; first by inversion H3; subst; apply values_no_reduce in Hred);
+              inversion H3; subst; 
+              destruct es => //; apply IHHred => //
+              )
+        ].
+    inversion H3; subst. destruct vs, es, es'0 => //.
+    + destruct vs.
+      2:{ inversion H5; subst. simpl in H0. repeat rewrite const_const in H0. done. }
+      inversion H5; subst.
+      destruct esnewest; first empty_list_no_reduce.
+      inversion H8; subst.
+      destruct esnewest => //.
+      clear - Hred.
+      exfalso.
+      lazymatch goal with
+    | _ : reduce _ _ ?esn _ _ _ |- _ => remember esn as ves
+    end.
+    induction Hred as [? ? ? ? H02 | | | | | | | | | | | | | | | | | | | | | | | | | | | | | | | | | | | | | | | | | ???????????? H02 H03 | ];
+        first destruct H02 as [| | | | | | | | | | | | | | | | | | | | | | | | | | | | | | | | | | | | | | | | | | ??? H01 ]; 
+        try (by inversion Heqves);
+        try (by destruct vs; try destruct vs; try destruct vs; try destruct vs; inversion Heqves);
+        try (by destruct ves; try destruct ves; try destruct ves; try destruct ves; inversion Heqves);
+        [ by move/lfilledP in H01; inversion H01; subst;
+          try (by do 4 destruct vs => //);
+          do 4 destruct bef => //
+        | move/lfilledP in H02; inversion H02; subst;
+          try (by do 4 destruct vs => //);
+          try (by do 4 destruct bef => //) ;
+          destruct vs;
+          first (
+              do 4 try (destruct es; first by inversion H3; subst; apply values_no_reduce in Hred);
+              inversion H3; subst; 
+              destruct es => //; apply IHHred => //
+              )
+        ].
+    inversion H3; subst.
+    done.
 Qed.
+
