theories/iris/helpers/reduce_det/reduce_det_testop.v
@@ -8,7 +8,36 @@ Lemma testop_i32_det c s f s' f' es testop:
     s' f' es [AI_basic (BI_const (VAL_int32 c)); AI_basic (BI_testop T_i32 testop)].
 Proof.
   move => Hred.
-  by only_one [AI_basic (BI_const (VAL_int32 c)) ; AI_basic (BI_testop T_i32 testop)] Hred.
+  only_one.
+  inversion H3; subst.
+  destruct vs; inversion H4; subst => //.
+  destruct esnewest; first empty_list_no_reduce.
+  inversion H1; subst.
+  destruct esnewest => //. 
+  clear -Hred.
+  lazymatch goal with
+  | _ : reduce _ _ ?esn _ _ _ |- _ => remember esn as ves
+  end.
+  exfalso. 
+  induction Hred as [? ? ? ? H02 | | | | | | | | | | | | | | | | | | | | | | | | | | | | | | | | | | | | | | | | | ???????????? H02 H03 | ];
+        first destruct H02 as [| | | | | | | | | | | | | | | | | | | | | | | | | | | | | | | | | | | | | | | | | | ??? H01 ]; 
+        try (by inversion Heqves);
+        try (by destruct vs; try destruct vs; try destruct vs; try destruct vs; inversion Heqves);
+        try (by destruct ves; try destruct ves; try destruct ves; try destruct ves; inversion Heqves);
+        [ by move/lfilledP in H01; inversion H01; subst;
+          try (by do 4 destruct vs => //);
+          do 4 destruct bef => //
+        | move/lfilledP in H02; inversion H02; subst;
+          try (by do 4 destruct vs => //);
+          try (by do 4 destruct bef => //);
+          destruct vs;
+          first (
+              do 4 try (destruct es; first by inversion H3; subst; apply values_no_reduce in Hred);
+              inversion H3; subst;
+              destruct es => //; apply IHHred => //
+              )
+        ].
+  inversion H3; subst => //.
 Qed.
 
 Lemma testop_i64_det c s f s' f' es testop:
@@ -17,5 +46,34 @@ Lemma testop_i64_det c s f s' f' es testop:
     s' f' es [AI_basic (BI_const (VAL_int64 c)); AI_basic (BI_testop T_i64 testop)].
 Proof.
   move => Hred.
-  by only_one [AI_basic (BI_const (VAL_int64 c)) ; AI_basic (BI_testop T_i64 testop)] Hred.
+   only_one.
+  inversion H3; subst.
+  destruct vs; inversion H4; subst => //.
+  destruct esnewest; first empty_list_no_reduce.
+  inversion H1; subst.
+  destruct esnewest => //. 
+  clear -Hred.
+  lazymatch goal with
+  | _ : reduce _ _ ?esn _ _ _ |- _ => remember esn as ves
+  end.
+  exfalso. 
+  induction Hred as [? ? ? ? H02 | | | | | | | | | | | | | | | | | | | | | | | | | | | | | | | | | | | | | | | | | ???????????? H02 H03 | ];
+        first destruct H02 as [| | | | | | | | | | | | | | | | | | | | | | | | | | | | | | | | | | | | | | | | | | ??? H01 ]; 
+        try (by inversion Heqves);
+        try (by destruct vs; try destruct vs; try destruct vs; try destruct vs; inversion Heqves);
+        try (by destruct ves; try destruct ves; try destruct ves; try destruct ves; inversion Heqves);
+        [ by move/lfilledP in H01; inversion H01; subst;
+          try (by do 4 destruct vs => //);
+          do 4 destruct bef => //
+        | move/lfilledP in H02; inversion H02; subst;
+          try (by do 4 destruct vs => //);
+          try (by do 4 destruct bef => //);
+          destruct vs;
+          first (
+              do 4 try (destruct es; first by inversion H3; subst; apply values_no_reduce in Hred);
+              inversion H3; subst;
+              destruct es => //; apply IHHred => //
+              )
+        ].
+  inversion H3; subst => //.
 Qed.
